var rename

theories/elpi.v
@@ -229,11 +229,13 @@ Variable p : program.
 From det Require Import finmap.
 Open Scope fset_scope.
 
+Notation bc := (bc u).
+
 (*SNIP: stepE *)
-Definition stepE fv t s a gl :=
-  let (fv', rs) := bc u p fv t s  in
+Definition stepE v0 t s a gl :=
+  let (v1, rs) := bc p v0 t s  in
   let rs_ca := save_alts a gl (r2a rs) in
-  (fv', rs_ca).
+  (v1, rs_ca).
 (*ENDSNIP: stepE *)
 
 (*prooftree: nurbp*)
@@ -241,37 +243,37 @@ Definition stepE fv t s a gl :=
 (*SNIP: nur_type*)
 Inductive runE : fvS -> Sigma -> goals ->  alts -> Sigma -> alts -> Prop :=
 (*ENDSNIP: nur_type*)
-| StopE s a fv : runE fv s [::] a s a
-| CutE s s1 a ca r gl fv : runE fv s gl ca s1 r -> runE fv s [:: (cut, ca) & gl] a s1 r
-| CallE s s1 al b bs gl r t ca fv fv': 
-    stepE fv t s al gl = (fv', [:: b & bs ]) -> 
-      runE fv' b.1 b.2 (bs++al) s1 r -> 
-        runE fv s [:: (call t, ca) & gl] al s1 r
-| FailE s s1 s2 t gl a al r ca fv fv': 
-    stepE fv t s al gl = (fv', [::]) -> 
-      runE fv' s1 a al s2 r ->   
-        runE fv s [:: (call t, ca) & gl] [:: (s1, a) & al] s2 r.
+| StopE s0 a v0 : runE v0 s0 [::] a s0 a
+| CutE s0 s1 a ca r gl v0 : runE v0 s0 gl ca s1 r -> runE v0 s0 [:: (cut, ca) & gl] a s1 r
+| CallE s0 s1 al b bs gl r t ca v0 v1: 
+    stepE v0 t s0 al gl = (v1, [:: b & bs ]) -> 
+      runE v1 b.1 b.2 (bs++al) s1 r -> 
+        runE v0 s0 [:: (call t, ca) & gl] al s1 r
+| FailE s0 s1 s2 t gl a al r ca v0 v1: 
+    stepE v0 t s0 al gl = (v1, [::]) -> 
+      runE v1 s1 a al s2 r ->   
+        runE v0 s0 [:: (call t, ca) & gl] [:: (s1, a) & al] s2 r.
 (*ENDSNIP: runE *)
 (*endprooftree: nurbp *)
 
-Lemma stepE_len fv t s a1 a2 gl:
-  size (stepE fv t s a1 gl).2 = size (stepE fv t s a2 gl).2.
+Lemma stepE_len v t s a1 a2 gl:
+  size (stepE v t s a1 gl).2 = size (stepE v t s a2 gl).2.
 Proof.
   rewrite/stepE; case: bc => //= _ b.
   by rewrite/save_alts !size_map.
 Qed.
 
-Lemma nur_consistent fv s G x xs1 xs2 s1 s2 :
-  runE fv s G x s1 xs1 -> runE fv s G x s2 xs2 -> xs1 = xs2 /\ s1 = s2.
+Lemma nur_consistent v s G x xs1 xs2 s1 s2 :
+  runE v s G x s1 xs1 -> runE v s G x s2 xs2 -> xs1 = xs2 /\ s1 = s2.
 Proof.
   move=> H; elim: H xs2 s2 => //; clear.
   - inversion 1 => //.
-  - move=> s a ca r gl fv H IH xs2.
+  - move=> s a ca r gl v H IH xs2.
     by inversion 1; subst; auto.
-  - move=> s s1 a b bs gl r t ca fv1 fv2 H H1 IH xs2 s2 H2.
+  - move=> s s1 a b bs gl r t ca v1 v2 H H1 IH xs2 s2 H2.
     apply: IH.
     inversion H2; subst => //; first by congruence.
-    have:= stepE_len fv1 t s al [:: (s3, a0)& al] gl.
+    have:= stepE_len v1 t s al [:: (s3, a0)& al] gl.
     by rewrite H10 H.
   - move=> s s1 s2 t gl a al r ca f1 f2 H H1 IH xs2 s3 H2.
     apply: IH.
